\documentclass[12pt, a4paper]{article}
\usepackage{titlesec}
\usepackage{lipsum}
\usepackage{amssymb}
\usepackage{amsmath}
\usepackage{bbm}
\usepackage[margin=1.3in]{geometry}
\usepackage[mathscr]{euscript}
\usepackage{tabto}
\usepackage{cancel}


\DeclareSymbolFont{rsfs}{U}{rsfs}{m}{n}
\DeclareSymbolFontAlphabet{\mathscrsfs}{rsfs}
\titlelabel{\thetitle.\quad}
\righthyphenmin=1000
\lefthyphenmin=1000


\begin{document}
\section*{Exercise 1.4}
\vspace{1em}

\subsection*{(a) Do you think that the value of $b$ depends on the variance of the measurement errors? Why?}
\begin{align*}
    &\beta = \frac{Cov(x, y)}{Var(x)}
\end{align*}
Variance of the measurement error contribute to the variance of $x$, hence value of $b$ is dependent on the variance of the measurement error.
\vspace{1em}


\subsection*{(b) Show that $b = \beta + \sum_{i=1}^n \frac{(x_i - \bar{x})(\epsilon_i - \bar{\epsilon})}{\sum_{i=1}^n(x_i - \bar{x})^2}$}
\begin{align*}
    b&=\frac{\sum_{i=1}^n(x_i-\bar{x})(y_i-\bar{y})}{\sum_{i=1}^n(x_i-\bar{x})^2}\\
    y_i-\bar{y}&= (\alpha + \beta x_i + \epsilon_i) - (\alpha + \beta \bar{x} + \bar{\epsilon})\\
    &=\beta(x_i-\bar{x}) - (\epsilon_i-\bar{\epsilon})\\\\
    b&=\frac{\sum_{i=1}^n(x_i-\bar{x})[\beta (x_i-\bar{x}) +  (\epsilon_i-\bar{\epsilon})]}{\sum_{i=1}^n(x_i-\bar{x})^2}\\
    & = \beta\frac{\sum_{i=1}^n(x_i-\bar{x})^2}{\sum_{i=1}^n(x_i-\bar{x})^2} + \frac{\sum_{i=1}^n(x_i-\bar{x})(\epsilon_i-\bar{\epsilon})}{\sum_{i=1}^n(x_i-\bar{x})^2}\\
    &= \beta + \frac{\sum_{i=1}^n(x_i-\bar{x})(\epsilon_i-\bar{\epsilon})}{\sum_{i=1}^n(x_i-\bar{x})^2}
\end{align*}
\vspace{1em}

\subsection*{(c) Show that $\epsilon_i = \epsilon_i^* - \beta v_i$}
\begin{align*}
    y_i = \alpha + \beta x_i^* + \epsilon_i^* & = \alpha + \beta x_i + \epsilon_i\\
    \alpha + \beta x_i^* + \epsilon_i^* & = \alpha + \beta (x_i^*+v_i) + \epsilon_i\\
    \alpha + \beta x_i^* + \epsilon_i^* & = \alpha + \beta x_i^* + \beta v_i + \epsilon_i\\
    \epsilon_i^* &= \beta v_i + \epsilon_i\\
    \epsilon_i &= \epsilon_i^*-\beta v_i\\
\end{align*}
\vspace{1em}

\subsection*{(d) Show that the covariance between $x_i$ and $\epsilon_i$ equal to $-\beta\sigma_v^2$}
\begin{align*}
    \text{Notes}\\
    &\sum_{i=1}^n(x_i^*-\bar{x}^*)(\epsilon_i^*-\bar{\epsilon}^*)=0\\
    &\sum_{i=1}^n(x_i^*-\bar{x}^*)(v_i -\bar{v})=0\\
    &\sum_{i=1}^n(v_i -\bar{v})(\epsilon_i^*-\bar{\epsilon}^*)=0\\\\
    Cov(x_i, \epsilon_i)&= \frac{\sum_{i=1}^n(x_i-\bar{x})(\epsilon_i-\bar{\epsilon})}{n-1}\\
    &= \frac{\sum_{i=1}^n(x_i^*+v_i-\bar{x}^* - \bar{v})(\epsilon_i^*-\beta v_i-\bar{\epsilon}^* + \beta \bar{v})}{n-1}\\
    &= \frac{\sum_{i=1}^n([x_i^*-\bar{x}^*] + [v_i -\bar{v}])([\epsilon_i^*-\bar{\epsilon}^*]- \beta[v_i -\bar{v}])}{n-1}\\
    &= -\frac{\sum_{i=1}^n(v_i -\bar{v})\beta(v_i -\bar{v})}{n-1}\\
    &= -\beta Var(v_i)\\
    &= -\beta \sigma_v^2
\end{align*}
\vspace{1em}

\subsection*{(e) Show that for large sample size $n$ we get $b - \beta = \frac{-\beta \sigma^2}{\sigma_*^2+\sigma_v^2}$}
\begin{align*}
    b - \beta &= \frac{Cov(x_i, \epsilon_i)}{Var(x_i)}\\
    &= \frac{-\beta \sigma_v^2}{Var(x_i^*+v_i)}\\
    &= \frac{-\beta \sigma_v^2}{Var(x_i^*)+Var(v_i)}\\
    &= \frac{-\beta \sigma_v^2}{\sigma_*^2+\sigma_v^2}
\end{align*}
\vspace{1em}

\subsection*{(f) Compute the approximate bias $(b-\beta)$ for $\beta = 1$ in the cases SN = 1, SN = 3, SN = 10 }
\begin{align*}
    b - \beta &= \frac{-\beta \sigma_v^2}{\sigma_*^2+\sigma_v^2}\\
    &= \frac{-\sigma_v^2}{\sigma_*^2+\sigma_v^2}\\
    &= -\frac{1}{\frac{\sigma_*^2}{\sigma_v^2}+1}\\
    &= -\frac{1}{SN+1}\\
\end{align*}
\begin{align*}
    &SN = 1 &&b -\beta = -\frac{1}{2}\\
    &SN = 3 &&b -\beta = -\frac{1}{4}\\
    &SN = 10 &&b -\beta = -\frac{1}{11}\\
\end{align*}
\vspace{1em}


\end{document}