\documentclass[12pt, a4paper]{article}
\usepackage{titlesec}
\usepackage{lipsum}
\usepackage{amssymb}
\usepackage{amsmath}
\usepackage{bbm}
\usepackage[margin=1.3in]{geometry}
\usepackage[mathscr]{euscript}
\usepackage{tabto}
\usepackage{cancel}


\DeclareSymbolFont{rsfs}{U}{rsfs}{m}{n}
\DeclareSymbolFontAlphabet{\mathscrsfs}{rsfs}
\titlelabel{\thetitle.\quad}
\righthyphenmin=1000
\lefthyphenmin=1000


\begin{document}
\section*{Text Exercise 4}
\vspace{1em}
\subsection*{Part (a)}
The answer to the third question ($d_i$) might depend on ommited factors. One possibility would be following another diet. Following another diet would affect both variable $d_i$ and the change in weight ($y_{i1} - y_{i0}$). This can result in an underestimation of significance of $d_i$. If the participant follow another diet, $d_i$ will be zero and ($y_{i1} - y_{i0}$) might be bigger than zero.\\
\vspace{1em}
\subsection*{Part (b)}
The two conditions can be rephrased as follows:
\begin{enumerate}
    \item $\frac{1}{n}Z'\varepsilon \to 0$: The variable $z$ representing the door-to-door advertising is not correlated to the residual of the OLS model in Part (a).
    \item $\frac{1}{n}Z'X \to Q\ne0$: The variable $z$ representing the door-to-door advertising is sufficiently correlated to the residual of the OLS model in Part (a).
\end{enumerate}
\vspace{1em}
\subsection*{Part (c)}
\begin{enumerate}
    \item $\frac{1}{n}Z'\varepsilon$: possible to test this statistically using Sargan test.
    \item $\frac{1}{n}Z'X$: possible to test statistically. Use t-test for coefficient significance for OLS with formula $X = \gamma Z + \eta$ where $\eta$ is the error term.
\end{enumerate}
\vspace{1em}
\subsection*{Part (d)}
\begin{align*}
    &\beta = (Z'X)^{-1}(Z'Y)\\
    &Z = \left(\begin{array}{cc}
        1&z_1\\
        1&z_2\\
        \vdots\\
        1&z_n
    \end{array}\right)\quad
    X = \left(\begin{array}{cc}
        1&d_1\\
        1&d_2\\
        \vdots\\
        1&d_n
    \end{array}\right)\quad
    Y = \left(\begin{array}{c}
        (y_{11} - y_{10})\\
        (y_{21} - y_{20})\\
        \vdots\\
        (y_{n1} - y_{n0})
    \end{array}\right)\quad\\\\
    &Z'X = 
    \left(\begin{array}{cccc}
        1&1&...&1\\
        z_1&z_2&...&z_n\\
    \end{array}\right)
    \left(\begin{array}{cc}
        1&d_1\\
        1&d_2\\
        \vdots\\
        1&d_n
    \end{array}\right) =
    \left(\begin{array}{c}
        n\\
        \sum_{i=1}^nz_id_i
    \end{array}\right)\\
    &(Z'X)^{-1} = 
    \left(\begin{array}{cc}
        \frac{1}{n}&\frac{1}{\sum_{i=1}^nz_id_i}
    \end{array}\right)\\\\
    &Z'Y = 
    \left(\begin{array}{cccc}
        1&1&...&1\\
        z_1&z_2&...&z_n\\
    \end{array}\right)
    \left(\begin{array}{c}
        (y_{11} - y_{10})\\
        (y_{21} - y_{20})\\
        \vdots\\
        (y_{n1} - y_{n0})
    \end{array}\right)=\left(\begin{array}{c}
        \sum_{i=1}^n(y_{i1} - y_{i0})\\
        \sum_{i=1}^nz_i(y_{i1} - y_{i0})
    \end{array}\right)
\end{align*}
\begin{align*}
    \therefore \beta &= \left(\begin{array}{cc}
        \frac{1}{n}&\frac{1}{\sum_{i=1}^nz_id_i}
    \end{array}\right)\left(\begin{array}{c}
        \sum_{i=1}^n(y_{i1} - y_{i0})\\
        \sum_{i=1}^nz_i(y_{i1} - y_{i0})
    \end{array}\right)\\
    &= \frac{\sum_{i=1}^n(y_{i1} - y_{i0})}{n} + \frac{\sum_{i=1}^nz_i(y_{i1} - y_{i0})}{\sum_{i=1}^nz_id_i}\\
    &= \Delta + \frac{\sum\limits_{k\in\{i\;|\;z_i=1\}}z_i(y_{i1} - y_{i0})+\overbrace{\sum_{k\in\{i\;|\;z_i=0\}}z_i(y_{i1} - y_{i0})}^{=0}}{\sum\limits_{k\in\{i\;|\;z_i=1\}}z_id_i+\underbrace{\sum_{k\in\{i\;|\;z_i=0\}}z_id_i}^{=0}}\\
    &= \Delta + \frac{\sum_{k\in\{i\;|\;z_i=1\}}z_i(y_{i1} - y_{i0})}{\sum_{k\in\{i\;|\;z_i=1\}}z_id_i}\\
    &= \Delta + \frac{\Delta^1}{\bar{d}^1}
\end{align*}
\vspace{1em}

\end{document}