\documentclass[12pt, a4paper]{article}
\usepackage{titlesec}
\usepackage{lipsum}
\usepackage{amssymb}
\usepackage{amsmath}
\usepackage{bbm}
\usepackage[margin=1.3in]{geometry}
\usepackage[mathscr]{euscript}
\usepackage{tabto}
\usepackage{cancel}


\DeclareSymbolFont{rsfs}{U}{rsfs}{m}{n}
\DeclareSymbolFontAlphabet{\mathscrsfs}{rsfs}
\titlelabel{\thetitle.\quad}
\righthyphenmin=1000
\lefthyphenmin=1000


\begin{document}
\section*{Text Exercise 5}
\vspace{1em}
\subsection*{Part (a)}
Answer:
\begin{align*}
    &\text{Given: }\\
    &\quad\beta_2 = 0.914\\
    &\quad\frac{\partial\text{Pr}[\text{resp}_i = 1]}{\partial\text{active}_i}\frac{\text{active}_i}{\text{Pr}[\text{resp}_i = 1]} = \text{Pr}[\text{resp}_i = 0] \text{active}_i\beta_2\\\\
    &\text{For age}=50,\;\text{active}=1,\;\text{male}=1:\\
    &\quad\text{Pr}[\text{resp}_i = 0] = \frac{1}{1+\text{exp}(\beta_0 + \beta_1\text{male}_i+\beta_2\text{active}_i+\beta_3\text{age}_i+\beta_4(\text{age}_i/10)^2)}\\
    &\quad\text{Pr}[\text{resp}_i = 0] =  0.240\\
    &\quad\text{Elasticity} = \text{Pr}[\text{resp}_i = 0] \text{active}_i\beta_2 = \bf 0.219\\\\
    &\text{For age}=50,\;\text{active}=0,\;\text{male}=1:\\
    &\quad\text{Elasticity} = \text{Pr}[\text{resp}_i = 0] \text{active}_i\beta_2 = \bf 0
\end{align*}
\vspace{1em}
\subsection*{Part (b)}
Answer:
\begin{align*}
    &\text{Given:}\\
    &\quad\frac{\text{Pr}[\text{resp}_i = 1\;|\;\text{active}_i=1] - \text{Pr}[\text{resp}_i = 1\;|\;\text{active}_i=0]}{\text{Pr}[\text{resp}_i = 1\;|\;\text{active}_i=0]}\\\\
    &\text{Let: }\\
    &\quad\gamma = \beta_0 + \beta_1\text{male}_i+\beta_2\text{active}_i+\beta_3\text{age}_i+\beta_4(\text{age}_i/10)^2\\\\
    &\text{Such that:}\\
    &\quad\text{Pr}[\text{resp}_i = 0] = \frac{1}{1+\text{exp}(\gamma + \beta_2\text{active}_i)}\\\\
    &\text{Therefore:}\\
    &\quad\frac{\text{Pr}[\text{resp}_i = 1\;|\;\text{active}_i=1] - \text{Pr}[\text{resp}_i = 1\;|\;\text{active}_i=0]}{\text{Pr}[\text{resp}_i = 1\;|\;\text{active}_i=0]}=\\
    &\quad\frac{\frac{\text{exp}(\gamma + \beta_2)}{1+\text{exp}(\gamma + \beta_2)}}{\frac{\text{exp}(\gamma)}{1+\text{exp}(\gamma)}} -1=\\
    &\quad\frac{\text{exp}(\gamma)\text{exp}(\beta_2)}{1+\text{exp}(\gamma + \beta_2)}\frac{1+\text{exp}(\gamma)}{\text{exp}(\gamma)} - 1=\\
    &\quad\frac{\text{exp}(\beta_2)+\text{exp}(\gamma + \beta_2)}{1+\text{exp}(\gamma + \beta_2)} - \frac{1+\text{exp}(\gamma + \beta_2)}{1+\text{exp}(\gamma + \beta_2)}=\\
    &\quad\frac{\text{exp}(\beta_2)}{1+\text{exp}(\gamma + \beta_2)} - \frac{1}{1+\text{exp}(\gamma + \beta_2)}=\\
    &\quad(\text{exp}(\beta_2)-1)\frac{1}{1+\text{exp}(\gamma + \beta_2)}=\\
    &\quad(\text{exp}(\beta_2)-1)\text{Pr}[\text{resp}_i = 0\;|\;\text{active}_i=1]
\end{align*}
\vspace{1em}
\subsection*{Part (c)}
Answer:
\begin{align*}
    &\text{Given: }\\
    &\quad\text{Elasticity} = (\text{exp}(\beta_2)-1)\text{Pr}[\text{resp}_i = 0\;|\;\text{active}_i=1]\\\\
    &\text{For age}=50,\;\text{active}=1,\;\text{male}=1:\\
    &\quad\text{Pr}[\text{resp}_i = 0\;|\;\text{active}_i=1] = \frac{1}{1+\text{exp}(\beta_0 + \beta_1\text{male}_i+\beta_2+\beta_3\text{age}_i+\beta_4(\text{age}_i/10)^2)}\\
    &\quad\text{Pr}[\text{resp}_i = 0\;|\;\text{active}_i=1] =  0.240\\
    &\quad\text{Elasticity} =(\text{exp}(\beta_2)-1)\text{Pr}[\text{resp}_i = 0\;|\;\text{active}_i=1] = \bf 0.358\\\\
\end{align*}
\vspace{1em}

\end{document}